Structure/BuildingBlocks.lean
@@ -18,61 +18,60 @@ universes u v
 
 namespace BuildingBlocks
 
-structure DependentFunctor where
+-- We start with abstractions of Π and Σ types where types and instances are replaced with structures.
+-- Although Σ may be redundant in theory, it is very important for our use case because bundled instances
+-- of type classes are Σ types.
+
+structure EncodedLambda where
 (S : Structure)
 (C : StructureFunctor S universeStructure)
 
-def makeDependentFunctor {S : Structure} (C : StructureFunctor S sortStructure) : DependentFunctor :=
+def toEncodedLambda {S : Structure} (C : StructureFunctor S sortStructure) : EncodedLambda :=
 ⟨S, compFun C sortToStructureFunctor⟩
 
-structure EncodedPiExpr (T : DependentFunctor) where
-(map (α : T.S) : (T.C α).U)
+structure EncodedPiExpr (L : EncodedLambda) where
+(map (α : L.S) : (L.C α).U)
 
-instance (T : DependentFunctor) : CoeFun (EncodedPiExpr T) (λ F => ∀ α : T.S, (T.C α).U) := ⟨EncodedPiExpr.map⟩
+instance (L : EncodedLambda) : CoeFun (EncodedPiExpr L) (λ f => ∀ α : L.S, (L.C α).U) := ⟨EncodedPiExpr.map⟩
 
--- TODO: Σ may be redundant because everything is built on Π/∀ in Lean.
-
-structure EncodedSigmaExpr (T : DependentFunctor) where
-(α : T.S)
-(x : (T.C α).U)
+structure EncodedSigmaExpr (L : EncodedLambda) where
+(α : L.S)
+(x : (L.C α).U)
 
 -- Every term of type `∀ x, C x` or `Σ' x, C x` where everything has structures and functors can be
 -- converted to an instance of `EncodedPiExpr` or `EncodedSigmaExpr`, respectively.
 
--- TODO: Figure out in which cases we can determine the functor properties of `C` automatically.
--- Easiest case: `C` does not actually depend on `x`, i.e. we have a function...
+def encodePiExpr    {α : Sort u} [h : HasStructure α] (C : StructureFunctor (defaultStructure α) sortStructure) (f : ∀  x : α, C x) :
+  EncodedPiExpr    (toEncodedLambda C) := ⟨f⟩
 
-def encodePiExpr    {α : Sort u} [h : HasStructure α] {C : StructureFunctor (defaultStructure α) sortStructure} (f : ∀  x : α, C x) :
-  EncodedPiExpr    (makeDependentFunctor C) := ⟨f⟩
-
-def encodeSigmaExpr {α : Sort u} [h : HasStructure α] {C : StructureFunctor (defaultStructure α) sortStructure} (f : Σ' x : α, C x) :
-  EncodedSigmaExpr (makeDependentFunctor C) := ⟨f.fst, f.snd⟩
+def encodeSigmaExpr {α : Sort u} [h : HasStructure α] (C : StructureFunctor (defaultStructure α) sortStructure) (s : Σ' x : α, C x) :
+  EncodedSigmaExpr (toEncodedLambda C) := ⟨s.fst, s.snd⟩
 
 
 
 -- We can define equivalences between such Π and Σ expressions. These fulfill the isomorphism axioms
--- and thus turn the types `EncodedPiExpr T` and `EncodedSigmaExpr T` into structures.
+-- and thus turn the types `EncodedPiExpr L` and `EncodedSigmaExpr L` into structures.
 
-def PiEquiv {T : DependentFunctor} (F G : EncodedPiExpr T) := DependentEquiv F.map G.map
+def PiEquiv {L : EncodedLambda} (f g : EncodedPiExpr L) := DependentEquiv f.map g.map
 
 namespace PiEquiv
 
-variable {T : DependentFunctor}
+variable {L : EncodedLambda}
 
-def refl  (F     : EncodedPiExpr T)                                     : PiEquiv F F :=
-DependentEquiv.refl  F.map
-def symm  {F G   : EncodedPiExpr T} (φ : PiEquiv F G)                   : PiEquiv G F :=
+def refl  (f     : EncodedPiExpr L)                                     : PiEquiv f f :=
+DependentEquiv.refl  f.map
+def symm  {f g   : EncodedPiExpr L} (φ : PiEquiv f g)                   : PiEquiv g f :=
 DependentEquiv.symm  φ
-def trans {F G H : EncodedPiExpr T} (φ : PiEquiv F G) (ψ : PiEquiv G H) : PiEquiv F H :=
+def trans {f g h : EncodedPiExpr L} (φ : PiEquiv f g) (ψ : PiEquiv g h) : PiEquiv f h :=
 DependentEquiv.trans φ ψ
 
-def piEquiv (F G : EncodedPiExpr T) := DependentEquiv.dependentEquiv F.map G.map
+def piEquiv (f g : EncodedPiExpr L) := DependentEquiv.dependentEquiv f.map g.map
 
 -- Unfortunately, uncommenting this line (after uncommenting DependentEquiv.dependentEquivHasIso first)
 -- causes Lean to hang indefinitely, so we have to copy and paste the code instead.
 --instance piEquivHasIso : HasIsomorphisms (@piEquiv T) := @DependentEquiv.dependentEquivHasIso T.S T.C.map
 
-instance piEquivHasIso : HasIsomorphisms (@piEquiv T) :=
+instance piEquivHasIso : HasIsomorphisms (@piEquiv L) :=
 { comp         := trans,
   congrArgComp := λ hφ hψ α => congrArgComp (hφ α) (hψ α),
   assoc        := λ φ ψ χ α => assoc        (φ α) (ψ α) (χ α),
@@ -85,14 +84,14 @@ instance piEquivHasIso : HasIsomorphisms (@piEquiv T) :=
   rightInv     := λ φ     α => rightInv     (φ α),
   invInv       := λ φ     α => invInv       (φ α),
   compInv      := λ φ ψ   α => compInv      (φ α) (ψ α),
-  idInv        := λ F     α => idInv        (F α) }
+  idInv        := λ f     α => idInv        (f α) }
 
 end PiEquiv
 
 open PiEquiv
 
-instance piHasStructure (T : DependentFunctor) : HasStructure (EncodedPiExpr T) := ⟨piEquiv⟩
-def piStructure (T : DependentFunctor) : Structure := ⟨EncodedPiExpr T⟩
+instance piHasStructure (L : EncodedLambda) : HasStructure (EncodedPiExpr L) := ⟨piEquiv⟩
+def piStructure (L : EncodedLambda) : Structure := ⟨EncodedPiExpr L⟩
 
 
 
@@ -102,51 +101,51 @@ def piStructure (T : DependentFunctor) : Structure := ⟨EncodedPiExpr T⟩
 -- we have an equivalence between the types such that `congrArgMap` maps one instance of the type
 -- class to the other.
 
-def SigmaEquiv {T : DependentFunctor} (F G : EncodedSigmaExpr T) :=
-Σ' e : F.α ≃ G.α, InstanceEquiv (T.C.congrArgMap e) F.x G.x
+def SigmaEquiv {L : EncodedLambda} (s t : EncodedSigmaExpr L) :=
+Σ' e : s.α ≃ t.α, InstanceEquiv (congrArgMap L.C e) s.x t.x
 
 namespace SigmaEquiv
 
-variable {T : DependentFunctor}
+variable {L : EncodedLambda}
 
-def refl  (F     : EncodedSigmaExpr T)                                           : SigmaEquiv F F :=
-let h₁ := InstanceEquiv.refl (setoidStructure (T.C F.α)) F.x;
-let h₂ := Setoid.symm (respectsId   T.C F.α);
-⟨IsEquivalence.refl  F.α,         InstanceEquiv.congrArg h₂ F.x F.x h₁⟩
+def refl  (s     : EncodedSigmaExpr L)                                           : SigmaEquiv s s :=
+let h₁ := InstanceEquiv.refl (setoidStructure (L.C s.α)) s.x;
+let h₂ := Setoid.symm (respectsId   L.C s.α);
+⟨IsEquivalence.refl  s.α,         InstanceEquiv.congrArg h₂ s.x s.x h₁⟩
 
-def symm  {F G   : EncodedSigmaExpr T} (φ : SigmaEquiv F G)                      : SigmaEquiv G F :=
-let h₁ := InstanceEquiv.symm (congrArgMap T.C φ.fst) F.x G.x φ.snd;
-let h₂ := Setoid.symm (respectsInv  T.C φ.fst);
-⟨IsEquivalence.symm  φ.fst,       InstanceEquiv.congrArg h₂ G.x F.x h₁⟩
+def symm  {s t   : EncodedSigmaExpr L} (φ : SigmaEquiv s t)                      : SigmaEquiv t s :=
+let h₁ := InstanceEquiv.symm (congrArgMap L.C φ.fst) s.x t.x φ.snd;
+let h₂ := Setoid.symm (respectsInv  L.C φ.fst);
+⟨IsEquivalence.symm  φ.fst,       InstanceEquiv.congrArg h₂ t.x s.x h₁⟩
 
-def trans {F G H : EncodedSigmaExpr T} (φ : SigmaEquiv F G) (ψ : SigmaEquiv G H) : SigmaEquiv F H :=
-let h₁ := InstanceEquiv.trans (congrArgMap T.C φ.fst) (congrArgMap T.C ψ.fst) F.x G.x H.x φ.snd ψ.snd;
-let h₂ := Setoid.symm (respectsComp T.C φ.fst ψ.fst);
-⟨IsEquivalence.trans φ.fst ψ.fst, InstanceEquiv.congrArg h₂ F.x H.x h₁⟩
+def trans {r s t : EncodedSigmaExpr L} (φ : SigmaEquiv r s) (ψ : SigmaEquiv s t) : SigmaEquiv r t :=
+let h₁ := InstanceEquiv.trans (congrArgMap L.C φ.fst) (congrArgMap L.C ψ.fst) r.x s.x t.x φ.snd ψ.snd;
+let h₂ := Setoid.symm (respectsComp L.C φ.fst ψ.fst);
+⟨IsEquivalence.trans φ.fst ψ.fst, InstanceEquiv.congrArg h₂ r.x t.x h₁⟩
 
 -- No need to compare `φ.snd` and `ψ.snd` because they are proofs.
-def SigmaEquivEquiv {F G : EncodedSigmaExpr T} (φ ψ : SigmaEquiv F G) := φ.fst ≈ ψ.fst
+def SigmaEquivEquiv {s t : EncodedSigmaExpr L} (φ ψ : SigmaEquiv s t) := φ.fst ≈ ψ.fst
 
 namespace SigmaEquivEquiv
 
-variable {F G : EncodedSigmaExpr T}
+variable {s t : EncodedSigmaExpr L}
 
-theorem refl  (φ     : SigmaEquiv F G)                                                     : SigmaEquivEquiv φ φ :=
+theorem refl  (φ     : SigmaEquiv s t)                                                     : SigmaEquivEquiv φ φ :=
 Setoid.refl  φ.fst
 
-theorem symm  {φ ψ   : SigmaEquiv F G} (e : SigmaEquivEquiv φ ψ)                           : SigmaEquivEquiv ψ φ :=
+theorem symm  {φ ψ   : SigmaEquiv s t} (e : SigmaEquivEquiv φ ψ)                           : SigmaEquivEquiv ψ φ :=
 Setoid.symm  e
 
-theorem trans {φ ψ χ : SigmaEquiv F G} (e : SigmaEquivEquiv φ ψ) (f : SigmaEquivEquiv ψ χ) : SigmaEquivEquiv φ χ :=
+theorem trans {φ ψ χ : SigmaEquiv s t} (e : SigmaEquivEquiv φ ψ) (f : SigmaEquivEquiv ψ χ) : SigmaEquivEquiv φ χ :=
 Setoid.trans e f
 
-instance sigmaEquivSetoid : Setoid (SigmaEquiv F G) := ⟨SigmaEquivEquiv, ⟨refl, symm, trans⟩⟩
+instance sigmaEquivSetoid : Setoid (SigmaEquiv s t) := ⟨SigmaEquivEquiv, ⟨refl, symm, trans⟩⟩
 
 end SigmaEquivEquiv
 
-def sigmaEquiv (F G : EncodedSigmaExpr T) : BundledSetoid := ⟨SigmaEquiv F G⟩
+def sigmaEquiv (s t : EncodedSigmaExpr L) : BundledSetoid := ⟨SigmaEquiv s t⟩
 
-instance sigmaEquivHasIso : HasIsomorphisms (@sigmaEquiv T) :=
+instance sigmaEquivHasIso : HasIsomorphisms (@sigmaEquiv L) :=
 { comp         := trans,
   congrArgComp := λ hφ hψ => congrArgComp hφ hψ,
   assoc        := λ φ ψ χ => assoc        φ.fst ψ.fst χ.fst,
@@ -159,23 +158,116 @@ instance sigmaEquivHasIso : HasIsomorphisms (@sigmaEquiv T) :=
   rightInv     := λ φ     => rightInv     φ.fst,
   invInv       := λ φ     => invInv       φ.fst,
   compInv      := λ φ ψ   => compInv      φ.fst ψ.fst,
-  idInv        := λ F     => idInv        F.α }
+  idInv        := λ s     => idInv        s.α }
 
 end SigmaEquiv
 
 open SigmaEquiv
 
-instance sigmaHasStructure (T : DependentFunctor) : HasStructure (EncodedSigmaExpr T) := ⟨@sigmaEquiv T⟩
-def sigmaStructure (T : DependentFunctor) : Structure := ⟨EncodedSigmaExpr T⟩
+instance sigmaHasStructure (L : EncodedLambda) : HasStructure (EncodedSigmaExpr L) := ⟨sigmaEquiv⟩
+def sigmaStructure (L : EncodedLambda) : Structure := ⟨EncodedSigmaExpr L⟩
+
+
+
+-- If we think of `SigmaEquiv` as defining our concept of isomorphism, we can actually _prove_ that
+-- isomorphisms between particular structures match their concrete definitions. This even works for
+-- structures that lack an obvious concept of "morphism".
+--
+-- We will call `EncodedSigmaExpr.α` the "type" and `EncodedSigmaExpr.x` the "instance" (that depends
+-- on the type). Correspondingly, `SigmaEquiv.fst` is the "type equivalence", and `SigmaEquiv.snd` is the
+-- corresponding "instance equivalence".
+
+namespace AbstractIsomorphism
+
+-- We would like to state our theorems not about the entire `SigmaEquiv` but about how the instance
+-- equivalence depends on the type equivalence.
+-- Whenever we do want to reason about the entire `SigmaEquiv`, `isoEquiv` will provide the desired
+-- result. Although `isoEquiv` is a _definition_ (of an equivalence), it can also be read as the theorem
+-- that the two types are equivalent.
+
+def HasIso {L : EncodedLambda} (s t : EncodedSigmaExpr L) (I : ∀ e : s.α ≃ t.α, Prop) :=
+∀ e : s.α ≃ t.α, InstanceEquiv (congrArgMap L.C e) s.x t.x ↔ I e
+
+def isoEquiv {L : EncodedLambda} {s t : EncodedSigmaExpr L} {I : ∀ e : s.α ≃ t.α, Prop} (h : HasIso s t I) :
+  SigmaEquiv s t ≃≃ Σ' e : s.α ≃ t.α, I e :=
+{ toFun    := λ ⟨h₁, h₂⟩ => ⟨h₁, (h h₁).mp  h₂⟩,
+  invFun   := λ ⟨h₁, h₂⟩ => ⟨h₁, (h h₁).mpr h₂⟩,
+  leftInv  := λ ⟨h₁, h₂⟩ => rfl,
+  rightInv := λ ⟨h₁, h₂⟩ => rfl }
+
+-- Degenerate case: If the instance does not actually depend on the type, an isomorphism is just an
+-- equivalence between the types together with an equivalence between the instances.
+
+def constantLambda (S T : Structure) : EncodedLambda := ⟨S, constFun T⟩
+
+namespace constantLambda
+
+variable (S T : Structure)
+
+-- This degenerate case is actually equivalent to `PProd S T`.
+
+def equivProd : EncodedSigmaExpr (constantLambda S T) ≃≃ PProd S.U T.U :=
+{ toFun    := λ ⟨x, y⟩ => ⟨x, y⟩,
+  invFun   := λ ⟨x, y⟩ => ⟨x, y⟩,
+  leftInv  := λ ⟨x, y⟩ => rfl,
+  rightInv := λ ⟨x, y⟩ => rfl }
+
+-- The theorem about the instance equivalence.
+
+theorem iso (s t : EncodedSigmaExpr (constantLambda S T)) :
+  HasIso s t (λ e => s.x ≈ t.x) :=
+λ e => Iff.refl (s.x ≈ t.x)
+
+-- For this particular case, we can also specialize `isoEquiv` a bit.
+
+def equiv (s t : EncodedSigmaExpr (constantLambda S T)) :
+  SigmaEquiv s t ≃≃ PProd (s.α ≃ t.α) (s.x ≈ t.x) :=
+{ toFun    := λ ⟨h₁, h₂⟩ => ⟨h₁, h₂⟩,
+  invFun   := λ ⟨h₁, h₂⟩ => ⟨h₁, h₂⟩,
+  leftInv  := λ ⟨h₁, h₂⟩ => rfl,
+  rightInv := λ ⟨h₁, h₂⟩ => rfl }
+
+end constantLambda
+
+-- While in this degenerate case, the left and right side could actually be arbitrary structures, in the
+-- following cases we will really consider the left side as a type, in particular we need to work with
+-- instances of this type.
+--
+-- Since in our generalized framework, the instances should actually be arbitrary structure, we represent
+-- the type not by an arbitrary structure but by an instance of `universeStructure`.
+
+-- The first such case is that the instance on the right is just a particular instance of the type on the
+-- left, i.e. we have a generalized "pointed type" structure. Obviously, in that case an isomorphism
+-- should transport the instance along the type equivalence.
+
+def instanceLambda : EncodedLambda := ⟨universeStructure, idFun⟩
+
+namespace instanceLambda
+
+def equivSigma : EncodedSigmaExpr instanceLambda ≃≃ Σ' S : Structure, S.U :=
+{ toFun    := λ ⟨S, x⟩ => ⟨S, x⟩,
+  invFun   := λ ⟨S, x⟩ => ⟨S, x⟩,
+  leftInv  := λ ⟨S, x⟩ => rfl,
+  rightInv := λ ⟨S, x⟩ => rfl }
+
+theorem iso (s t : EncodedSigmaExpr instanceLambda) :
+  HasIso s t (λ e => e.toFun s.x ≈ t.x) :=
+λ e => setoidInstanceEquiv (congrArgMap instanceLambda.C e) s.x t.x
+
+end instanceLambda
+
+end AbstractIsomorphism
+
+
 
 
 
 -- If we have an `Equiv` with a type that has a structure, we can transport the structure along
 -- that `Equiv`.
 
--- TODO: Do we still need this?
+-- TODO: Do we still need this, or is the use case completely covered by `toTypeClassFunctor`?
 
-instance hasEquivalentStructure {α : Sort u} {β : Sort v} [h : HasStructure β] (e : Equiv α β) : HasStructure α :=
+instance hasEquivalentStructure {α : Sort u} {β : Sort v} [h : HasStructure β] (e : α ≃≃ β) : HasStructure α :=
 { M := λ a b => h.M (e.toFun a) (e.toFun b),
   h := { comp         := h.h.comp,
          congrArgComp := h.h.congrArgComp,
@@ -201,14 +293,56 @@ instance hasEquivalentStructure {α : Sort u} {β : Sort v} [h : HasStructure β
 -- We can do that by providing equivalences between `C α` and `D α`, where `D` is already known to be a
 -- functor from `sortStructure` to `sortStructure`.
 
-def TypeClass := Type u → Type v
+def TypeClass := Sort u → Sort v
 
-def TypeClassEquiv (C D : TypeClass) := ∀ α, Equiv (C α) (D α)
+def TypeClassEquiv (C D : TypeClass) := ∀ α, C α ≃≃ D α
 
 def TypeClassFunctor := StructureFunctor sortStructure sortStructure
 
-def toTypeClassFunctor (C : TypeClass) (D : TypeClassFunctor) (φ : TypeClassEquiv C D.map) : TypeClassFunctor :=
-proxyFunctor C D φ
+instance : CoeFun TypeClassFunctor (λ F => Sort u → Sort v) := ⟨λ F => F.map⟩
+
+class StructuralTypeClass (C : TypeClass) where
+(F : TypeClassFunctor)
+(φ : TypeClassEquiv C F.map)
+
+def toTypeClassFunctor (C : TypeClass) [h : StructuralTypeClass C] : TypeClassFunctor :=
+proxyFunctor C h.F h.φ
+
+
+
+-- A bundled instance of a type class is just a dependent pair. If the type class is a functor, we can
+-- build an `EncodedSigmaExpr`, which has a structure.
+
+def bundledStructure (C : TypeClass) [h : StructuralTypeClass C] := sigmaStructure (toEncodedLambda (toTypeClassFunctor C))
+
+def bundled (C : TypeClass) [h : StructuralTypeClass C] (α : Sort u) (x : C α) : bundledStructure C := ⟨α, x⟩
+
+def bundledType     {C : TypeClass} [h : StructuralTypeClass C] (S : bundledStructure C) : Sort u := S.α
+def bundledInstance {C : TypeClass} [h : StructuralTypeClass C] (S : bundledStructure C) : C S.α  := S.x
+
+
+
+-- This lets us define isomorphism of two instances of a type class as equivalence of the corresponding
+-- bundled structures.
+
+def Isomorphism {C : TypeClass} [h : StructuralTypeClass C] (α : Sort u) (x : C α) (β : Sort u) (y : C β) :=
+bundled C α x ≃ bundled C β y
+
+-- From an isomorphism, we can recover the `Equiv` of the types and the condition on the instances.
+
+def isoTypeEquiv {C : TypeClass} [h : StructuralTypeClass C] {α : Sort u} {x : C α} {β : Sort u} {y : C β} (e : Isomorphism α x β y) :
+  α ≃≃ β :=
+e.fst
+
+def isoInstanceEquiv {C : TypeClass} [h : StructuralTypeClass C] {α : Sort u} {x : C α} {β : Sort u} {y : C β} (e : Isomorphism α x β y) :
+  C α ≃ C β :=
+congrArgMap (toTypeClassFunctor C) e.fst
+
+theorem isoCondition {C : TypeClass} [h : StructuralTypeClass C] {α : Sort u} {x : C α} {β : Sort u} {y : C β} (e : Isomorphism α x β y) :
+-- TODO: Write in terms of `congrArgMap D e.fst`.
+  (isoInstanceEquiv e).toFun x = y :=
+-- TODO: Need to undo `sortToStructureFunctor`.
+sorry --e.snd
 
 end BuildingBlocks
 
