Structure/Examples.lean
@@ -21,6 +21,10 @@ open BuildingBlocks
 
 
 
+universe u
+
+
+
 namespace Examples
 
 -- As the simplest example of a type class, let us consider `Inhabited` from `Prelude`, which gives a
@@ -30,15 +34,30 @@ namespace Examples
 -- `Inhabited` should be, we need to show that the function `Inhabited : Sort _ → Sort _` is a
 -- `StructureFunctor`.
 -- The easiest way to do this is to observe that the content of `Inhabited α` is actually a single
--- instance of `α`, so we have an `Equiv` between `Inhabited α` and `α`. That gives us a `TypeClassEquiv`
--- between `Inhabited` and `id`, and then `toTypeClassFunctor` will return the required functor.
+-- instance of `α`, so we have an `Equiv` between `Inhabited α` and `α`. Using this `Equiv`, the type
+-- class `Inhabited` becomes an instance (!) of the type class `StructuralTypeClass`.
 
-def inhabitedEquivInstance (α : Sort u) : Equiv (Inhabited α) α :=
+namespace Inhabited
+
+def inhabitedEquiv (α : Type u) : Equiv (Inhabited α) α :=
 { toFun    := λ ⟨x⟩ =>  x,
   invFun   := λ  x  => ⟨x⟩,
   leftInv  := λ ⟨x⟩ => rfl,
   rightInv := λ  x  => rfl }
 
-def inhabitedFunctor := toTypeClassFunctor Inhabited idFun inhabitedEquivInstance
+instance : StructuralTypeClass Inhabited := ⟨idFun, inhabitedEquiv⟩
+
+-- This gives us a definition of when two inhabited types are isomorphic.
+
+def Iso (α β : Type u) [h₁ : Inhabited α] [h₂ : Inhabited β] := Isomorphism α h₁ β h₂
+
+-- Let's check whether that definition is actually the correct one.
+
+theorem isoMapsBasePoint {α β : Type u} [h₁ : Inhabited α] [h₂ : Inhabited β] (e : Iso α β) :
+  (isoTypeEquiv e).toFun h₁.default = h₂.default :=
+let h := isoCondition e;
+sorry
+
+end Inhabited
 
 end Examples
